<?xml version="1.0" encoding="UTF-8"?>
<rdf:RDF
	xmlns:skos="http://www.w3.org/2004/02/skos/core#"
	xmlns:cc="http://web.resource.org/cc/"
	xmlns:dctype="http://purl.org/dc/dcmitype/"
	xmlns:dct="http://purl.org/dc/terms/"
	xmlns:vann="http://purl.org/vocab/vann/"
	xmlns:dc="http://purl.org/dc/elements/1.1/"
	xmlns:rdf="http://www.w3.org/1999/02/22-rdf-syntax-ns#"
	xmlns:rdfs="http://www.w3.org/2000/01/rdf-schema#"
	xmlns:owl="http://www.w3.org/2002/07/owl#"
	xmlns:xsd="http://www.w3.org/2001/XMLSchema#"
	xmlns:multi-tenant="http://purl.org/vocab/multi-tenant-configuration/schema#"
	>
	<owl:Ontology rdf:about="" dc:date="2009-05-13">
		<dc:title xml:lang="en">Multi-Tenant Configuration Schema</dc:title>
		<rdfs:comment xml:lang="en">
			The Multi-Tenant Configuration Schema provides 
    	</rdfs:comment>
		<dc:identifier>http://purl.org/vocab/multi-tenant-configuration/schema-20090513</dc:identifier>
		<dct:isVersionOf rdf:resource="#"/>
		<dc:creator>Rob Styles</dc:creator>
		<dc:rights>Copyright Â© 2009 Talis Information Ltd</dc:rights>
		<vann:preferredNamespaceUri>http://purl.org/vocab/multi-tenant-configuration/schema#</vann:preferredNamespaceUri>
		<vann:preferredNamespacePrefix>multi-tenant</vann:preferredNamespacePrefix>
		<vann:example rdf:resource="schema-diagram.html" />
		<dct:hasFormat>
			<dctype:Text rdf:about="http://purl.org/vocab/multi-tenant-configuration/schema-20090513.html">
				<dc:format>
					<dct:IMT>
						<rdf:value>text/html</rdf:value>
						<rdfs:label xml:lang="en">HTML</rdfs:label>
					</dct:IMT>
				</dc:format>
			</dctype:Text>
		</dct:hasFormat>
		<dct:hasFormat>
			<dctype:Text rdf:about="http://purl.org/vocab/multi-tenant-configuration/schema-20090513.rdf">
				<dc:format>
					<dct:IMT>
						<rdf:value>application/rdf+xml</rdf:value>
						<rdfs:label xml:lang="en">RDF</rdfs:label>
					</dct:IMT>
				</dc:format>
			</dctype:Text>
		</dct:hasFormat>
		<dct:issued>2009-05-13</dct:issued>
		<skos:historyNote rdf:value="First draft of the ontology published" dc:date="2009-05-13" dc:creator="Rob Styles"/>
	</owl:Ontology>
	<cc:Work rdf:about="">
		<cc:license rdf:resource="http://creativecommons.org/licenses/by/2.0/uk/"/>
	</cc:Work>
	<cc:License rdf:about="http://creativecommons.org/licenses/by/2.0/uk/">
		<cc:permits rdf:resource="http://web.resource.org/cc/Reproduction"/>
		<cc:permits rdf:resource="http://web.resource.org/cc/Distribution"/>
		<cc:requires rdf:resource="http://web.resource.org/cc/Notice"/>
		<cc:requires rdf:resource="http://web.resource.org/cc/Attribution"/>
		<cc:permits rdf:resource="http://web.resource.org/cc/DerivativeWorks"/>
	</cc:License>
	
	<rdfs:Class rdf:about="#Customer">
		<rdfs:label xml:lang="en">Customer</rdfs:label>
		<rdfs:comment xml:lang="en">A customer represents your customer. They may have zero or more tenancies. We need to consider how this class relates to foaf:Agent and possibly other ontologies describing CRM models.</rdfs:comment>
		<rdfs:isDefinedBy rdf:resource="#"/>
		<dct:issued>2009-05-13</dct:issued>
	</rdfs:Class>

	<rdfs:Class rdf:about="#Tenancy">
		<rdfs:label xml:lang="en">Tenancy</rdfs:label>
		<rdfs:comment xml:lang="en">A tenancy represents the area or part of the service that is owned by a particular customer. A customer may own more than one tenancy.</rdfs:comment>
		<rdfs:isDefinedBy rdf:resource="#"/>
		<dct:issued>2009-05-13</dct:issued>
	</rdfs:Class>

	<rdfs:Class rdf:about="#TenancyType">
		<rdfs:label xml:lang="en">Tenancy Type</rdfs:label>
		<rdfs:comment xml:lang="en">Tenancy Types allow the tenancies of different systems to be distinguished within a single graph. You should define a tenancy type within your own namespace for each multi-tenant application you are describing tenancies for.</rdfs:comment>
		<rdfs:isDefinedBy rdf:resource="#"/>
		<dct:issued>2009-05-13</dct:issued>
	</rdfs:Class>

	<rdfs:Class rdf:about="#Subscription">
		<rdfs:label xml:lang="en">Subscription</rdfs:label>
		<rdfs:comment xml:lang="en">Subscription resources track the periods for which a customer has subscribed to the service and at what subscription level.</rdfs:comment>
		<rdfs:isDefinedBy rdf:resource="#"/>
		<dct:issued>2009-05-13</dct:issued>
	</rdfs:Class>

	<rdfs:Class rdf:about="#SubscriptionLevel">
		<rdfs:label xml:lang="en">Subscription Level</rdfs:label>
		<rdfs:comment xml:lang="en">Subscription Level resources allow your application to tailor its feature set based on subscription levels you define within your own namespace.</rdfs:comment>
		<rdfs:isDefinedBy rdf:resource="#"/>
		<dct:issued>2009-05-13</dct:issued>
	</rdfs:Class>

	<rdfs:Class rdf:about="#Feature">
		<rdfs:label xml:lang="en">Feature</rdfs:label>
		<rdfs:comment xml:lang="en">You can describe features within your own namespace, relating them to different subscription levels.</rdfs:comment>
		<rdfs:isDefinedBy rdf:resource="#"/>
		<dct:issued>2009-05-13</dct:issued>
	</rdfs:Class>

	<rdf:Property rdf:about="#customer">
		<rdfs:label xml:lang="en">Customer</rdfs:label>
		<rdfs:comment>The customer property links a Tenancy with the Customer who owns it.</rdfs:comment>
		<rdfs:domain rdf:resource="#Tenancy"/>
		<rdfs:range rdf:resource="#Customer"/>
		<owl:inverseOf rdf:resource="#tenancy"/>
		<dct:issued>2009-05-13</dct:issued>
		<rdfs:isDefinedBy rdf:resource="#"/>
	</rdf:Property>

	<rdf:Property rdf:about="#tenancy">
		<rdfs:label xml:lang="en">Tenancy</rdfs:label>
		<rdfs:comment>The tenancy property links a Customer with the tenancies they own.</rdfs:comment>
		<rdfs:domain rdf:resource="#Tenancy"/>
		<rdfs:range rdf:resource="#Customer"/>
		<owl:inverseOf rdf:resource="#customer"/>
		<dct:issued>2009-05-13</dct:issued>
		<rdfs:isDefinedBy rdf:resource="#"/>
	</rdf:Property>
	
	<rdf:Property rdf:about="#tenancyType">
		<rdfs:label xml:lang="en">Tenancy Type</rdfs:label>
		<rdfs:comment>The type of tenancy this resource describes.</rdfs:comment>
		<rdfs:domain rdf:resource="#Tenancy"/>
		<rdfs:range rdf:resource="#TenancyType"/>
		<dct:issued>2009-05-13</dct:issued>
		<rdfs:isDefinedBy rdf:resource="#"/>
	</rdf:Property>

	<rdf:Property rdf:about="#subscription">
		<rdfs:label xml:lang="en">Subscription</rdfs:label>
		<rdfs:comment>A subscription that enables the use of this tenancy.</rdfs:comment>
		<rdfs:domain rdf:resource="#Tenancy"/>
		<rdfs:range rdf:resource="#TenancyType"/>
		<dct:issued>2009-05-13</dct:issued>
		<rdfs:isDefinedBy rdf:resource="#"/>
	</rdf:Property>

	<rdf:Property rdf:about="#createdAt">
		<rdfs:label xml:lang="en">Created</rdfs:label>
		<rdfs:comment>The date on which the tenancy was created. Managing this allows multiple tenancies to be displayed in time order.</rdfs:comment>
		<rdfs:domain rdf:resource="#Tenancy"/>
		<rdfs:range rdf:resource="http://www.w3.org/2001/XMLSchema#dateTime"/>
		<dct:issued>2009-05-13</dct:issued>
		<rdfs:isDefinedBy rdf:resource="#"/>
	</rdf:Property>

	<rdf:Property rdf:about="#enabled">
		<rdfs:label xml:lang="en">Enabled</rdfs:label>
		<rdfs:comment>A simple boolean value that allows a tenancy to be enabled or disabled entirely.</rdfs:comment>
		<rdfs:domain rdf:resource="#Tenancy"/>
		<rdfs:range rdf:resource="http://www.w3.org/2001/XMLSchema#boolean"/>
		<dct:issued>2009-05-13</dct:issued>
		<rdfs:isDefinedBy rdf:resource="#"/>
	</rdf:Property>

	<rdf:Property rdf:about="#subscriptionLevel">
		<rdfs:label xml:lang="en">Subscription Level</rdfs:label>
		<rdfs:comment>The level at which the customer has subscribed to this tenancy.</rdfs:comment>
		<rdfs:domain rdf:resource="#Subscription"/>
		<rdfs:range rdf:resource="http://www.w3.org/2001/XMLSchema#dateTime"/>
		<dct:issued>2009-05-13</dct:issued>
		<rdfs:isDefinedBy rdf:resource="#"/>
	</rdf:Property>

	<rdf:Property rdf:about="#validUntil">
		<rdfs:label xml:lang="en">Valid Until</rdfs:label>
		<rdfs:comment>The date on which a subscription expires.</rdfs:comment>
		<rdfs:domain rdf:resource="#Subscription"/>
		<rdfs:range rdf:resource="http://www.w3.org/2001/XMLSchema#dateTime"/>
		<dct:issued>2009-05-13</dct:issued>
		<rdfs:isDefinedBy rdf:resource="#"/>
	</rdf:Property>

	<rdf:Property rdf:about="#validFrom">
		<rdfs:label xml:lang="en">Valid From</rdfs:label>
		<rdfs:comment>The date from which a subscription is valid.</rdfs:comment>
		<rdfs:domain rdf:resource="#Subscription"/>
		<rdfs:range rdf:resource="http://www.w3.org/2001/XMLSchema#dateTime"/>
		<dct:issued>2009-05-13</dct:issued>
		<rdfs:isDefinedBy rdf:resource="#"/>
	</rdf:Property>

	<rdf:Property rdf:about="#allowedFeature">
		<rdfs:label xml:lang="en">Allowed Feature</rdfs:label>
		<rdfs:comment>A feature that is allowed for subscriptions at this subscription level. This allows for a white-listing approach to feature control.</rdfs:comment>
		<rdfs:domain rdf:resource="#SubscriptionLevel"/>
		<rdfs:range rdf:resource="#Feature"/>
		<dct:issued>2009-05-13</dct:issued>
		<rdfs:isDefinedBy rdf:resource="#"/>
	</rdf:Property>

	<rdf:Property rdf:about="#disallowedFeature">
		<rdfs:label xml:lang="en">Disallowed Feature</rdfs:label>
		<rdfs:comment>A feature that is not allowed for subscriptions at this subscription level. This allows for a black-listing approach to feature control.</rdfs:comment>
		<rdfs:domain rdf:resource="#SubscriptionLevel"/>
		<rdfs:range rdf:resource="#Feature"/>
		<dct:issued>2009-05-13</dct:issued>
		<rdfs:isDefinedBy rdf:resource="#"/>
	</rdf:Property>

</rdf:RDF>
