<!DOCTYPE rdf:RDF [
    <!ENTITY changeset  "http://purl.org/vocab/changeset/schema#" >
    <!ENTITY xsd  "http://www.w3.org/2001/XMLSchema#" >
    <!ENTITY foaf  "http://xmlns.com/foaf/0.1/" >
    <!ENTITY owl  "http://www.w3.org/2002/07/owl#" >
    <!ENTITY cc  "http://web.resource.org/cc/" >
    <!ENTITY vocabid  "http://purl.org/vocab/changeset/schema-20060321" >
	  <!ENTITY skos "http://www.w3.org/2004/02/skos/core#">
]>
<rdf:RDF xmlns:rdf="http://www.w3.org/1999/02/22-rdf-syntax-ns#"
    xmlns:owl="http://www.w3.org/2002/07/owl#" 
    xmlns:dc="http://purl.org/dc/elements/1.1/" 
    xmlns:vann="http://purl.org/vocab/vann/" 
    xmlns:dct="http://purl.org/dc/terms/" 
    xmlns:dctype="http://purl.org/dc/dcmitype/" 
    xmlns:cc="http://web.resource.org/cc/"
    xmlns:skos="http://www.w3.org/2004/02/skos/core#"
    xmlns:rdfs="http://www.w3.org/2000/01/rdf-schema#">

  <owl:Ontology rdf:about="" dc:date="2006-03-21">
    <dc:title xml:lang="en">Changesets</dc:title>
    <rdfs:comment xml:lang="en">
      This vocabulary defines a set of terms for describing changes to resource descriptions.
    </rdfs:comment>
    <rdfs:comment xml:lang="en">
      The vocabulary introduces the notion of a ChangeSet which encapsulates the delta between two versions of a 
      resource description. In this context a resource description is the set of triples that in some way comprise a 
      description of a resource. The delta is represented by two sets of triples: additions and removals. A ChangeSet can be used to 
      modify a resource description by first removing all triples from the description that are in the removals set and
      adding the triples in the additions set.
    </rdfs:comment>


		<dc:identifier>&vocabid;</dc:identifier>
		<dct:isVersionOf rdf:resource="&changeset;"/>
		<dc:creator>Sam Tunnicliffe</dc:creator>
		<dc:creator>Ian Davis &lt;http://purl.org/NET/iand&gt;</dc:creator>
		<dc:rights>Copyright © 2005 Talis Information Ltd.</dc:rights>
		<dct:replaces rdf:resource="http://purl.org/vocab/changesets/schema-20051214"/>
		<vann:preferredNamespaceUri>&changeset;</vann:preferredNamespaceUri>
		<vann:preferredNamespacePrefix>cs</vann:preferredNamespacePrefix>
		<vann:example rdf:resource="./changesets-example-20060321.html" dc:title="A Simple ChangeSet"/>
		<vann:example rdf:resource="./changesets-example2-20060321.html" dc:title="Linked ChangeSets"/>
		<vann:example rdf:resource="./changesets-example3-20060321.html" dc:title="Implementing Undo With ChangeSets"/>

		<dct:hasFormat>
			<dctype:Text rdf:about="&vocabid;.html">
				<dc:format>
					<dct:IMT>
						<rdf:value>text/html</rdf:value>
						<rdfs:label xml:lang="en">HTML</rdfs:label>
					</dct:IMT>
				</dc:format>
			</dctype:Text>
		</dct:hasFormat>

		<dct:hasFormat>
			<dctype:Text rdf:about="&vocabid;.rdf">
				<dc:format>
					<dct:IMT>
						<rdf:value>application/rdf+xml</rdf:value>
						<rdfs:label xml:lang="en">RDF</rdfs:label>
					</dct:IMT>
				</dc:format>
			</dctype:Text>
		</dct:hasFormat>

    <dct:issued>2005-12-14</dct:issued>
    <skos:changeNote rdf:value="Improved documentation" dc:date="2006-03-21" dc:creator="Ian Davis"/>
    <skos:historyNote rdf:value="Introduced statement property" dc:date="2006-03-21" dc:creator="Ian Davis"/>
  </owl:Ontology>

  <owl:ObjectProperty rdf:about="&changeset;statement">
    <rdfs:label xml:lang="en">statement</rdfs:label>        
    <skos:definition xml:lang="en">a triple included in this set of changes</skos:definition>
    <rdfs:domain rdf:resource="http://purl.org/vocab/changeset/schema#ChangeSet"/>
    <rdfs:isDefinedBy rdf:resource="&changeset;"/>
    <rdfs:range rdf:resource="http://www.w3.org/1999/02/22-rdf-syntax-ns#Statement"/>
    <dct:issued>2006-03-21</dct:issued>
  </owl:ObjectProperty>


  <owl:ObjectProperty rdf:about="&changeset;addition">
    <rdfs:label xml:lang="en">addition</rdfs:label>        
    <skos:definition xml:lang="en">a triple to be added to the resource description</skos:definition>
    <rdfs:comment xml:lang="en">
      By convention the subject of the triple being added should be the same as the subjectOfChange
    </rdfs:comment>
    <rdfs:subPropertyOf rdf:resource="&changeset;statement"/>
    <rdfs:domain rdf:resource="http://purl.org/vocab/changeset/schema#ChangeSet"/>
    <rdfs:isDefinedBy rdf:resource="&changeset;"/>
    <rdfs:range rdf:resource="http://www.w3.org/1999/02/22-rdf-syntax-ns#Statement"/>
    <dct:issued>2005-12-14</dct:issued>
    <skos:changeNote rdf:value="Added definitition and documentation" dc:date="2006-03-21" dc:creator="Ian Davis"/>
    <skos:historyNote rdf:value="Made owl:ObjectProperty" dc:date="2006-03-21" dc:creator="Ian Davis"/>
    <skos:historyNote rdf:value="Made a sub-property of statement" dc:date="2006-03-21" dc:creator="Ian Davis"/>
  </owl:ObjectProperty>


  <owl:ObjectProperty rdf:about="&changeset;removal">
    <rdfs:label xml:lang="en">removal</rdfs:label>        
    <skos:definition xml:lang="en">a triple to be removed from the resource description</skos:definition>
    <rdfs:comment xml:lang="en">
      By convention the subject of the triple being removed should be the same as the subjectOfChange
    </rdfs:comment>
    <rdfs:subPropertyOf rdf:resource="&changeset;statement"/>
    <rdfs:domain rdf:resource="http://purl.org/vocab/changeset/schema#ChangeSet"/>
    <rdfs:isDefinedBy rdf:resource="&changeset;"/>
    <rdfs:range rdf:resource="http://www.w3.org/1999/02/22-rdf-syntax-ns#Statement"/>
    <dct:issued>2005-12-14</dct:issued>
    <skos:changeNote rdf:value="Added definitition and documentation" dc:date="2006-03-21" dc:creator="Ian Davis"/>
    <skos:historyNote rdf:value="Made owl:ObjectProperty" dc:date="2006-03-21" dc:creator="Ian Davis"/>
    <skos:historyNote rdf:value="Made a sub-property of statement" dc:date="2006-03-21" dc:creator="Ian Davis"/>
  </owl:ObjectProperty>


  <owl:ObjectProperty rdf:about="&changeset;subjectOfChange">
    <rdfs:label xml:lang="en">subjectOfChange</rdfs:label>        
    <skos:definition xml:lang="en">the resource to which this set of changes applies</skos:definition>
    <rdfs:domain rdf:resource="http://purl.org/vocab/changeset/schema#ChangeSet"/>
    <rdfs:isDefinedBy rdf:resource="&changeset;"/>
    <rdfs:range rdf:resource="http://www.w3.org/2000/01/rdf-schema#Resource"/>
    <dct:issued>2005-12-14</dct:issued>
    <skos:changeNote rdf:value="Added definitition and documentation" dc:date="2006-03-21" dc:creator="Ian Davis"/>
    <skos:historyNote rdf:value="Made owl:ObjectProperty" dc:date="2006-03-21" dc:creator="Ian Davis"/>
  </owl:ObjectProperty>


  <owl:ObjectProperty rdf:about="&changeset;precedingChangeSet">
    <rdfs:label xml:lang="en">precedingChangeSet</rdfs:label>        
    <skos:definition xml:lang="en">the changeset that immediately precedes this one</skos:definition>
    <rdfs:comment xml:lang="en">
      This property can be used to build a history of changes to a particular resource description. The first
      ChangeSet in the history will have no precedingChangeSet property. Each subsequent ChangeSet added
      to the history references the preceding one resulting in a singly-linked list of changes.  Care must be taken
      not to introduce cycles in the history.
    </rdfs:comment>
    <rdfs:comment xml:lang="en">
      In systems that assume a closed world, the most recent ChangeSet for a particular resource description 
      can be discovered by looking for the ChangeSet that is not the value of a precedingChangeSet property. 
      Conversely, the earliest ChangeSet is the one that is not the subject of a precedingChangeSet property.
    </rdfs:comment>
    <rdfs:domain rdf:resource="http://purl.org/vocab/changeset/schema#ChangeSet"/>
    <rdfs:isDefinedBy rdf:resource="&changeset;"/>
    <rdfs:range rdf:resource="http://purl.org/vocab/changeset/schema#ChangeSet"/>
    <dct:issued>2005-12-14</dct:issued>
    <skos:changeNote rdf:value="Added definitition and documentation" dc:date="2006-03-21" dc:creator="Ian Davis"/>
    <skos:historyNote rdf:value="Made owl:ObjectProperty" dc:date="2006-03-21" dc:creator="Ian Davis"/>
  </owl:ObjectProperty>


  <owl:DatatypeProperty rdf:about="&changeset;createdDate">
    <rdfs:label xml:lang="en">createdDate</rdfs:label>      
    <skos:definition xml:lang="en">the date that the changeset was created</skos:definition>
    <rdfs:comment xml:lang="en">
      The date should be in W3CDTF format
    </rdfs:comment>
    <rdfs:domain rdf:resource="http://purl.org/vocab/changeset/schema#ChangeSet"/>
    <rdfs:subPropertyOf rdf:resource="http://purl.org/dc/elements/1.1/date"/>
    <rdfs:isDefinedBy rdf:resource="&changeset;"/>
    <dct:issued>2005-12-14</dct:issued>
    <skos:historyNote rdf:value="Made owl:DatatypeProperty" dc:date="2006-03-21" dc:creator="Ian Davis"/>
  </owl:DatatypeProperty>


  <owl:DatatypeProperty rdf:about="&changeset;changeReason">
    <rdfs:label xml:lang="en">changeReason</rdfs:label>
    <skos:definition xml:lang="en">a  short, human readable description of the purpose for the changeset</skos:definition>
    <rdfs:domain rdf:resource="http://purl.org/vocab/changeset/schema#ChangeSet"/>
    <rdfs:isDefinedBy rdf:resource="&changeset;"/>
    <rdfs:range rdf:resource="http://www.w3.org/2000/01/rdf-schema#Literal"/>
    <dct:issued>2005-12-14</dct:issued>
    <skos:historyNote rdf:value="Made owl:DatatypeProperty" dc:date="2006-03-21" dc:creator="Ian Davis"/>
  </owl:DatatypeProperty>  


  <owl:DatatypeProperty rdf:about="&changeset;creatorName">
    <rdfs:label xml:lang="en">creatorName</rdfs:label>
    <skos:definition xml:lang="en">the name of the entity responsible for creating the changeset</skos:definition>
    <rdfs:domain rdf:resource="http://purl.org/vocab/changeset/schema#ChangeSet"/>
    <rdfs:isDefinedBy rdf:resource="&changeset;"/>
    <rdfs:range rdf:resource="http://www.w3.org/2000/01/rdf-schema#Literal"/>
    <dct:issued>2005-12-14</dct:issued>
    <skos:historyNote rdf:value="Made owl:DatatypeProperty" dc:date="2006-03-21" dc:creator="Ian Davis"/>
  </owl:DatatypeProperty>


  <rdfs:Class rdf:about="&changeset;ChangeSet">
    <rdfs:label xml:lang="en">ChangeSet</rdfs:label>
    <skos:definition xml:lang="en">The encapsulation of a delta between two versions of a resource description</skos:definition>
    <rdfs:isDefinedBy rdf:resource="&changeset;"/>
    <dct:issued>2005-12-14</dct:issued>
    <skos:changeNote rdf:value="Improved documentation" dc:date="2006-03-21" dc:creator="Ian Davis"/>
    <skos:historyNote rdf:value="Added property cardinality restrictions" dc:date="2006-03-21" dc:creator="Ian Davis"/>

    <rdfs:subClassOf>
      <owl:Class>
        <owl:intersectionOf>
          <owl:Restriction>
            <owl:onProperty rdf:resource="&changeset;statement"/>
            <owl:minCardinality rdf:datatype="&xsd;nonNegativeInteger">1</owl:minCardinality>
          </owl:Restriction>
          <owl:Restriction>
            <owl:onProperty rdf:resource="&changeset;previousChangeSet"/>
            <owl:maxCardinality rdf:datatype="&xsd;nonNegativeInteger">1</owl:maxCardinality>
          </owl:Restriction>
          <owl:Restriction>
            <owl:onProperty rdf:resource="&changeset;subjectOfChange"/>
            <owl:maxCardinality rdf:datatype="&xsd;nonNegativeInteger">1</owl:maxCardinality>
          </owl:Restriction>
          <owl:Restriction>
            <owl:onProperty rdf:resource="&changeset;createdDate"/>
            <owl:maxCardinality rdf:datatype="&xsd;nonNegativeInteger">1</owl:maxCardinality>
          </owl:Restriction>
          <owl:Restriction>
            <owl:onProperty rdf:resource="&changeset;creatorName"/>
            <owl:maxCardinality rdf:datatype="&xsd;nonNegativeInteger">1</owl:maxCardinality>
          </owl:Restriction>
          <owl:Restriction>
            <owl:onProperty rdf:resource="&changeset;changeReason"/>
            <owl:maxCardinality rdf:datatype="&xsd;nonNegativeInteger">1</owl:maxCardinality>
          </owl:Restriction>
        </owl:intersectionOf>
      </owl:Class>
    </rdfs:subClassOf>
  </rdfs:Class>
</rdf:RDF>